SystemFD.lean
@@ -16,8 +16,10 @@ import SystemFD.Metatheory.Progress
 
 import SystemFD.Evaluator.Soundness
 import SystemFD.Evaluator
--- import SystemFD.Algorithm.Soundness1
--- import SystemFD.Algorithm.Soundness2
+
+import SystemFD.Algorithm.TypeMatch
+import SystemFD.Algorithm.Soundness1
+import SystemFD.Algorithm.Soundness2
 
 
 import SystemFD.Examples.Boolean
