SystemFD/Algorithm/TypeMatch.lean
@@ -292,153 +292,65 @@ case _ h =>
 theorem prefix_type_match_sound :
   prefix_type_match Γ A B = .some T ->
   PrefixTypeMatch Γ A B T
-:= by
-intros h;
-unfold prefix_type_match at h; simp at h
-rw [Option.bind_eq_some] at h
-cases h; case _ ξ h =>
-cases h; case _ h1 h2 =>
-rw [Option.bind_eq_some] at h2; simp at h2
-cases h2; case _ x h2 =>
-cases h2; case _ h2 h3 =>
-cases h3; case _ h3 h4 =>
-cases h3; case _ h3 h5 =>
-cases h3; case _ h3 h6 =>
-cases h2; case _ sp h2 =>
-  generalize Aspdef : A.to_telescope = Asp at *
-  generalize Bspdef : B.to_telescope = Bsp at *
-  cases Asp; case _ τ sR =>
-  cases Bsp; case _ τ' sT =>
-    simp at *
-    replace h6 := Term.eq_of_beq h6
-    replace h3 := Term.eq_of_beq h3
-    apply prefix_type_match_sound_lemma
-      (Eq.symm Aspdef) (Eq.symm Bspdef) (Eq.symm h1)
-    rw [<-h4]; simp; apply h3
-    rw [<-Subst.apply_compose_commute] at h6
-    apply h6; apply Eq.symm h2
-    apply h5
-
-theorem valid_ctor_sound_lemma :
-  (τ, R) = Term.to_telescope A ->
-  .some (x, sp) = Term.neutral_form R ->
-  x' = x - τ.length ->
-  x = x' + τ.length ->
-  (Γ d@ x').is_datatype ->
-  ValidCtor Γ A
-:= by
-intro h1 h2 h3 h4 h5
-induction A generalizing τ R x sp x' Γ <;> try simp at h1
-any_goals try (
-  case _ =>
-    cases h1; case _ e1 e2 =>
-      subst e1; subst e2
-      constructor; unfold ValidHeadVariable
-      apply Exists.intro _; apply And.intro
-      apply h2; subst h3; simp; apply h5
-)
-case _ v t1 t2 ih1 ih2 =>
-  cases v <;> try simp at h1
-  any_goals try (
-    cases h1; case _ e1 e2 =>
-      subst e1; subst e2
-      constructor; unfold ValidHeadVariable
-      apply Exists.intro _; apply And.intro
-      apply h2; subst h3; simp; apply h5
-  )
-  case _ =>
-    generalize Bdef : t2.to_telescope = B at *
-    cases B; case _ γ rB =>
-    cases h1; case _ h1 h2 =>
-      subst h1; subst h2; simp at *
-      have lem1 : x' + 1 = x - γ.length := by omega
-      have lem2 : x = x' + 1 + γ.length := by omega
-      apply ValidCtor.all
-      apply ih2 rfl rfl h2 lem1 lem2
-      simp; rw [Frame.is_datatype_stable]; apply h5
-  case _ =>
-    generalize Bdef : t2.to_telescope = B at *
-    cases B; case _ γ rB =>
-    cases h1; case _ h1 h2 =>
-      subst h1; subst h2; simp at *
-      have lem1 : x' + 1 = x - γ.length := by omega
-      have lem2 : x = x' + 1 + γ.length := by omega
-      apply ValidCtor.arrow
-      apply ih2 rfl rfl h2 lem1 lem2
-      simp; rw [Frame.is_datatype_stable]; apply h5
+:= by sorry
+-- intros h;
+-- unfold prefix_type_match at h; simp at h
+-- rw [Option.bind_eq_some] at h
+-- cases h; case _ ξ h =>
+-- cases h; case _ h1 h2 =>
+-- rw [Option.bind_eq_some] at h2; simp at h2
+-- cases h2; case _ x h2 =>
+-- cases h2; case _ h2 h3 =>
+-- cases h3; case _ h3 h4 =>
+-- cases h3; case _ h3 h5 =>
+-- cases h3; case _ h3 h6 =>
+-- cases h2; case _ sp h2 =>
+--   generalize Aspdef : A.to_telescope = Asp at *
+--   generalize Bspdef : B.to_telescope = Bsp at *
+--   cases Asp; case _ τ sR =>
+--   cases Bsp; case _ τ' sT =>
+--     simp at *
+--     replace h6 := Term.eq_of_beq h6
+--     replace h3 := Term.eq_of_beq h3
+--     apply prefix_type_match_sound_lemma
+--       (Eq.symm Aspdef) (Eq.symm Bspdef) (Eq.symm h1)
+--     rw [<-h4]; simp; apply h3
+--     rw [<-Subst.apply_compose_commute] at h6
+--     apply h6; apply Eq.symm h2
+--     apply h5
 
 theorem valid_ctor_sound : valid_ctor Γ A = .some () -> ValidCtor Γ A := by
-intro h
-unfold valid_ctor at h; simp at h
-rw [Option.bind_eq_some] at h; simp at h
-cases h; case _ a h =>
-cases h; case _ h1 h2 =>
-cases h2; case _ h2 h3 =>
-  generalize Aspdef : A.to_telescope = Asp at *
-  cases Asp; case _ τ sA =>
-  cases h1; case _ sp h1 =>
-    simp at *
-    apply valid_ctor_sound_lemma
-      (Eq.symm Aspdef) (Eq.symm h1) rfl h2 h3
-
-theorem valid_insttype_sound_lemma :
-  (τ, R) = Term.to_telescope A ->
-  .some (x, sp) = Term.neutral_form R ->
-  x' = x - τ.length ->
-  x = x' + τ.length ->
-  (Γ d@ x').is_opent ->
-  ValidInstType Γ A
-:= by
-intro h1 h2 h3 h4 h5
-induction A generalizing τ R x sp x' Γ <;> try simp at h1
-any_goals try (
-  case _ =>
-    cases h1; case _ e1 e2 =>
-      subst e1; subst e2
-      constructor; unfold ValidHeadVariable
-      apply Exists.intro _; apply And.intro
-      apply h2; subst h3; simp; apply h5
-)
-case _ v t1 t2 ih1 ih2 =>
-  cases v <;> try simp at h1
-  any_goals try (
-    cases h1; case _ e1 e2 =>
-      subst e1; subst e2
-      constructor; unfold ValidHeadVariable
-      apply Exists.intro _; apply And.intro
-      apply h2; subst h3; simp; apply h5
-  )
-  case _ =>
-    generalize Bdef : t2.to_telescope = B at *
-    cases B; case _ γ rB =>
-    cases h1; case _ h1 h2 =>
-      subst h1; subst h2; simp at *
-      have lem1 : x' + 1 = x - γ.length := by omega
-      have lem2 : x = x' + 1 + γ.length := by omega
-      apply ValidInstType.all
-      apply ih2 rfl rfl h2 lem1 lem2
-      simp; rw [Frame.is_opent_stable]; apply h5
-  case _ =>
-    generalize Bdef : t2.to_telescope = B at *
-    cases B; case _ γ rB =>
-    cases h1; case _ h1 h2 =>
-      subst h1; subst h2; simp at *
-      have lem1 : x' + 1 = x - γ.length := by omega
-      have lem2 : x = x' + 1 + γ.length := by omega
-      apply ValidInstType.arrow
-      apply ih2 rfl rfl h2 lem1 lem2
-      simp; rw [Frame.is_opent_stable]; apply h5
+intro h; induction Γ, A using valid_ctor.induct;
+case _ ih =>
+  unfold valid_ctor at h;
+  replace ih := ih h;
+  apply ValidCtor.arrow ih;
+case _ ih =>
+  unfold valid_ctor at h;
+  replace ih := ih h;
+  apply ValidCtor.all ih;
+case _ =>
+  unfold valid_ctor at h;
+  simp at h; rw[Option.bind_eq_some] at h;
+  cases h; case _ w h =>
+  simp at h; have h1 := h.1; symm at h1; have h2 := h.2;
+  apply ValidCtor.refl; unfold ValidHeadVariable; apply Exists.intro w;
+  apply And.intro h1 (by simp; apply h2)
 
 theorem valid_insttype_sound : valid_insttype Γ A = .some () -> ValidInstType Γ A := by
-intro h
-unfold valid_insttype at h; simp at h
-rw [Option.bind_eq_some] at h; simp at h
-cases h; case _ a h =>
-cases h; case _ h1 h2 =>
-cases h2; case _ h2 h3 =>
-  generalize Aspdef : A.to_telescope = Asp at *
-  cases Asp; case _ τ sA =>
-  cases h1; case _ sp h1 =>
-    simp at *
-    apply valid_insttype_sound_lemma
-      (Eq.symm Aspdef) (Eq.symm h1) rfl h2 h3
+intro h; induction Γ, A using valid_insttype.induct;
+case _ ih =>
+  unfold valid_insttype at h;
+  replace ih := ih h;
+  apply ValidInstType.arrow ih;
+case _ ih =>
+  unfold valid_insttype at h;
+  replace ih := ih h;
+  apply ValidInstType.all ih;
+case _ =>
+  unfold valid_insttype at h;
+  simp at h; rw[Option.bind_eq_some] at h;
+  cases h; case _ w h =>
+  simp at h; have h1 := h.1; symm at h1; have h2 := h.2;
+  apply ValidInstType.refl; unfold ValidHeadVariable; apply Exists.intro w;
+  apply And.intro h1 (by simp; apply h2)
